\documentclass[12pt]{article}
\usepackage{amsmath}
\usepackage{graphicx}
\newcommand{\myvec}[1]{\begin{matrix} #1 \end{matrix}}

\title{ signals and systems
\vspace{1cm}

Gate2023-ee-Q46}
\author{EE23BTECH11014- Devarakonda Guna vaishnavi}

\begin{document}
\maketitle

Consider the state-space description of an LTI system with matrices
\begin{align*}
A = \begin{bmatrix} \myvec 0 & 1\\ \-1 & -2\end{bmatrix}, \quad 
B = \begin{bmatrix} \myvec0 \\ 1 \end{bmatrix}, \quad 
C = \begin{bmatrix} \myvec 3 & -2 \end{bmatrix}, \quad 
D = \begin{bmatrix} \myvec 1 \end{bmatrix}
\end{align*}

For the input, $\sin(\omega t)$, $\omega > 0$, the value of $\omega$ for which the steady-state output of the system will be zero, is \underline{\hspace{2cm}} (Round off to the nearest integer).\\
solution:
\begin{table}[h!]
    \centering
    \input{tables/table.tex}
    \caption{Input Parameters}
    \label{table:}
\end{table}

Transfer function given by:
\begin{align}
T.F &= C\begin{bmatrix} \myvec sI-A  \\    \end{bmatrix}^{-1}B + D\label{eq:gate46-1}\\
\begin{bmatrix} \myvec sI-A  \\    \end{bmatrix}&= \begin{bmatrix}\myvec s & -1 \\ \myvec 1  & s+2 \end{bmatrix}\label{eq:gate46-2}\\
\begin{bmatrix} \myvec sI - A \\   \end{bmatrix}^{-1}&=\begin{bmatrix} s & -1\\ \myvec 1& s+2 \end{bmatrix}^{-1}\label{eq:gate46-3}\\
\begin{bmatrix} \myvec sI - A \\   \end{bmatrix}^{-1}&=\frac{1}{s(s+2)+1}\begin{bmatrix} \myvec s+2 & 1 \\ \myvec -1 & s \end{bmatrix}\begin{bmatrix} \myvec 0 \\ 1 \label{eq:gate46-4} \end{bmatrix}
\end{align}
\vspace{1cm}

 Referencing from equation \eqref{eq:gate46-4}, equation \eqref{eq:gate46-1} becomes 

\begin{align}
T.F&=\begin{bmatrix} \myvec 3/s^2+2s+1 & -2/s^2+2s+1 \\  \end{bmatrix}  
\begin{bmatrix} \myvec s+2 & 1 \\  -1 & s \end{bmatrix}\begin{bmatrix} \myvec 0 \\ 1 \end{bmatrix} +1 \\
&=\begin{bmatrix} \myvec 3/s^2+2s+1 & -2/s^2+2s+1  \\ \end{bmatrix}\begin{bmatrix}
\myvec 0\\ 1 \end{bmatrix}+1\\
&=\frac{s^2 + 4}{s^2 + 2s + 1}\\
H(S)&=T.F\\
H(S)&=\frac{s^2 + 4}{s^2+2s+1}\label{eq:gate46-8}
\end{align}

Substituting $s=j\omega$ in equation \eqref{eq:gate46-8}.

\begin{align}
H(j\omega)=\frac{4-(\omega)^2}{1+2j\omega-(\omega)^2}
\end{align}

Steady state output of system is zero.

\begin{align}
4-(\omega)^2&=0\\
\omega&=2rad/sec
\end{align}

\end{document}




    






